# This is a draft RDF vocabulary for representing spatial data sets in INSPIRE as RDF. This vocabulary has been created using the "Guidelines for the RDF encoding of spatial data" (http://inspire-eu-rdf.github.io/inspire-rdf-guidelines).
#
# The use of RDF is optional and does not supersede or replace the requirements regarding encoding specified in Clause 9 of the INSPIRE Data Specifications. This optional encoding is intended to support the e-government and open data community in Europe, which is increasingly looking at RDF to represent data.
#
# This is a draft version. It has limitations and is expected to contain errors. Please report any issues or concerns in GitHub (https://github.com/inspire-eu-rdf/inspire-rdf-vocabularies/issues).
#
# ------------------------------
#
#
# This ontology contains classes and properties that have been derived from the INSPIRE "Hydro - Network" application schema.
#
# During the derivation, the following mappings, alignments, and omissions have been applied:
# - Mappings:
#   - Code list values are mapped to skos:Concept.
#
# - Alignments (through subsumption):
#   - Spatial object types are aligned with gsp:Feature.
#
# - Omissions: none
#
# ------------------------------
#
#
@prefix hy:    <http://inspire.ec.europa.eu/ont/hy#> .
@prefix hy-n:  <http://inspire.ec.europa.eu/ont/hy-n#> .
@prefix iso19150-2: <http://def.isotc211.org/iso19150/-2/2012/base#> .
@prefix gsp:   <http://www.opengis.net/ont/geosparql#> .
@prefix rdf:   <http://www.w3.org/1999/02/22-rdf-syntax-ns#> .
@prefix owl:   <http://www.w3.org/2002/07/owl#> .
@prefix xsd:   <http://www.w3.org/2001/XMLSchema#> .
@prefix skos:  <http://www.w3.org/2004/02/skos/core#> .
@prefix rdfs:  <http://www.w3.org/2000/01/rdf-schema#> .
@prefix net:   <http://inspire.ec.europa.eu/ont/net#> .
@prefix base:  <http://inspire.ec.europa.eu/ont/base#> .

hy-n:WatercourseSeparatedCrossing
        a                 owl:Class ;
        rdfs:comment      "NOTE The crossing may legitimately break a no-intersection quality rule."@en ;
        rdfs:isDefinedBy  <http://inspire.ec.europa.eu/featureconcept/WatercourseSeparatedCrossing> ;
        rdfs:subClassOf   hy:HydroObject , net:GradeSeparatedCrossing , gsp:Feature ;
        skos:definition   "An element in the hydrographic network used to indicate non-interacting crossing of watercourse links separated by level."@en .

hy-n:HydroNode.hydroNodeCategory
        a                owl:ObjectProperty ;
        rdfs:domain      hy-n:HydroNode ;
        rdfs:range       skos:Concept ;
        rdfs:seeAlso     <http://inspire.ec.europa.eu/codelist/HydroNodeCategoryValue> ;
        skos:definition  "Nature of the hydro node."@en .

<http://inspire.ec.europa.eu/ont/hy-n>
        a                owl:Ontology ;
        owl:imports      <https://github.com/inspire-eu-rdf/inspire-rdf-vocabularies/blob/master/base/base.ttl> , <http://www.opengis.net/ont/geosparql> , <http://www.w3.org/2004/02/skos/core> , <http://def.isotc211.org/iso19150/-2/2012/base> , <http://inspire.ec.europa.eu/ont/hy> , <https://github.com/inspire-eu-rdf/inspire-rdf-vocabularies/blob/master/net/net.ttl> ;
        owl:versionIRI   "http://inspire.ec.europa.eu/ont/hy-n/4.0" ;
        owl:versionInfo  "4.0" ;
        skos:definition  "The Network application schema contains spatial objects associated with a connected hydrographic network representation of waterways, lakes etc. This is required primarily for the 'spatial analysis and modelling' Use Case."@en .

hy-n:WatercourseLink.length
        a                owl:DatatypeProperty ;
        rdfs:domain      hy-n:WatercourseLink ;
        rdfs:range       base:Measure ;
        skos:definition  "Length of network segment."@en .

hy-n:HydroNode  a         owl:Class ;
        rdfs:comment      "NOTE May represent a physical confluence, bifurcation/confluence/vanishing point etc, or it may be associated with a hydrographic point of interest or facility."@en ;
        rdfs:isDefinedBy  <http://inspire.ec.europa.eu/featureconcept/HydroNode> ;
        rdfs:subClassOf   hy:HydroObject , net:Node , gsp:Feature ;
        skos:definition   "A node within the hydrographic network."@en .

hy-n:WatercourseLinkSequence
        a                 owl:Class ;
        rdfs:isDefinedBy  <http://inspire.ec.europa.eu/featureconcept/WatercourseLinkSequence> ;
        rdfs:subClassOf   hy:HydroObject , net:LinkSequence , gsp:Feature ;
        skos:definition   "A sequence of watercourse links representing a non-branching path through a hydrographic network."@en .

hy-n:WatercourseLink  a   owl:Class ;
        rdfs:comment      "NOTE A watercourse link may be fictitious, with no direct correspondence to a real-world object and included only to ensure a closed network.\r\n\r\nEXAMPLE Fictitious examples:\r\n- virtual network segment in coastal water area\r\n- virtual network segment in lake area\r\n- virtual network segment in river to connect tributary\r\n- virtual network segment in transitional water area"@en ;
        rdfs:isDefinedBy  <http://inspire.ec.europa.eu/featureconcept/WatercourseLink> ;
        rdfs:subClassOf   hy:HydroObject , net:Link , gsp:Feature ;
        skos:definition   "A segment of a watercourse within a hydrographic network."@en .

hy-n:WatercourseLink.flowDirection
        a                owl:ObjectProperty ;
        rdfs:domain      hy-n:WatercourseLink ;
        rdfs:range       skos:Concept ;
        rdfs:seeAlso     <http://inspire.ec.europa.eu/codelist/LinkDirectionValue> ;
        skos:definition  "Direction of water flow in the segment relative to digitisation of segment geometry."@en .
